\section{Part 2: Monovariable Control}

\subsection{Problem 1}

\begin{subequations}
		\begin{align*}
		\tilde V_d &= K_{pp} (\tilde p_c - \tilde p) - K_{pd} \dot {\tilde {p}}\\
		\ddot {\tilde p} &= K_1 (K_{pp} (\tilde p_c - \tilde p) - K_{pd} \dot {\tilde {p}})\\
		\ddot {\tilde p} &= K_1 K_{pp} \tilde p_c - K_1 K_{pp} \tilde p - K_1 K_{pd} \dot {\tilde p}
		\end{align*}	
\end{subequations}
We take the laplace transform:
\begin{subequations}
		\begin{align*}
		s^2 \hat{\tilde{p}} &= K_1 K_{pp} \hat{\tilde {p_c}} - K_1 K_{pp} \hat{\tilde p} - K_1 K_{pd} s \hat {\tilde p} \\
		(s^2 + s K_1 K_{pd} + K_1 K_{pp})\tilde{p} &= K_1 K_{pp} \tilde{p_c} \\
		\frac{\tilde{p}}{\tilde {p_c}} &= \frac{K_1 K_{pp}}{s^2 + s K_1 K_{pd} + K_1 K_{pp}}
		\end{align*}	
\end{subequations}